Interop printer: Most of the structure for Low* generation

src/arch/x64/interop/Main.ml
@@ -1,4 +1,5 @@
 open Interop_Printer
 
 let _ = print_string (translate_vale Linux X86 memcpy)
+let _ = print_newline()
 let _ = print_string (translate_lowstar memcpy)
